src/dafny/utils/Eth2Types.dfy
@@ -43,11 +43,9 @@ module Eth2Types {
     type Seq32Byte = x:seq<byte> | |x| == 32 witness timeSeq(0 as byte, 32)
     // SEQ_EMPTY_32_BYTES
 
-    datatype Uint256WithByteLength = Uint256WithByteLength(n:uint256,byteLength:nat)
-
-    type CorrectUint256WithByteLength = u:Uint256WithByteLength |   && u.n as nat < power2(u.byteLength * 8)
-                                                                    && 1 <= u.byteLength <= 32
-                                                                    witness Uint256WithByteLength(0,1)
+    type CorrectUint256WithByteLength = u:(uint256, nat) |  && u.0 as nat < power2(u.1 * 8)
+                                                            && 1 <= u.1 <= 32
+                                                            witness (0,1)
 
     // type Uint256WithByteLength = x:(uint256,nat) | && x.0 as nat < power2(x.1 * 8)
     //                                            && 1 <= x.1 <= 32 
@@ -68,94 +66,94 @@ module Eth2Types {
         |   Container(fl: seq<Serialisable>)
 
     type Uint = s:Serialisable |    s.Uint?
-                                    witness Uint(Uint256WithByteLength(0,1))
+                                    witness Uint((0,1))
     
 
     // The assert is required to for Dafny to verify that the provided witness
     // respects the constraint imposed by the existential quantifier
     type Uint8 = s:Uint |   assert  Equal<uint256>(0,0);
-                            && exists x:uint8 :: Equal<uint256>(s.n.n, x as uint256)
-                            && s.n.byteLength == 1
-                            witness Uint(Uint256WithByteLength(0,1))
+                            && exists x:uint8 :: Equal<uint256>(s.n.0, x as uint256)
+                            && s.n.1 == 1
+                            witness Uint((0,1))
 
     type Uint16 = s:Uint |  assert  Equal<uint256>(0,0);
-                            && exists x:uint16 :: Equal<uint256>(s.n.n, x as uint256)
-                            && s.n.byteLength == 2
-                            witness Uint(Uint256WithByteLength(0,2))   
+                            && exists x:uint16 :: Equal<uint256>(s.n.0, x as uint256)
+                            && s.n.1 == 2
+                            witness Uint((0,2))   
 
     type Uint32 = s:Uint |  assert  Equal<uint256>(0,0);
-                            && exists x:uint32 :: Equal<uint256>(s.n.n, x as uint256)
-                            && s.n.byteLength == 4
-                            witness Uint(Uint256WithByteLength(0,4))
+                            && exists x:uint32 :: Equal<uint256>(s.n.0, x as uint256)
+                            && s.n.1 == 4
+                            witness Uint((0,4))
  
 
     type Uint64 = s:Uint |  assert  Equal<uint256>(0,0);
                             // castUin64ToUint256 is probaly only required
                             // becaue uint256 is currently defined using power2
-                            && exists x:uint64 :: Equal<uint256>(s.n.n, castUin64ToUint256(x))
-                            && s.n.byteLength == 8
-                            witness Uint(Uint256WithByteLength(castUin64ToUint256(0),8))
+                            && exists x:uint64 :: Equal<uint256>(s.n.0, castUin64ToUint256(x))
+                            && s.n.1 == 8
+                            witness Uint((castUin64ToUint256(0),8))
 
     type Uint128 = s:Uint | assert  Equal<uint256>(0,0);
                             // castUi1284ToUint256 is probaly only required
                             // becaue uint256 is currently defined using power2
-                            && exists x:uint128 :: Equal<uint256>(s.n.n, castUin128ToUint256(x))
-                            && s.n.byteLength == 16
-                            witness Uint(Uint256WithByteLength(castUin128ToUint256(0),16))   
+                            && exists x:uint128 :: Equal<uint256>(s.n.0, castUin128ToUint256(x))
+                            && s.n.1 == 16
+                            witness Uint((castUin128ToUint256(0),16))   
 
     type Uint256 = s:Uint |  assert  Equal<uint256>(0,0);
-                            && exists x:uint256 :: Equal<uint256>(s.n.n, x as uint256)
-                            && s.n.byteLength == 32
-                            witness Uint(Uint256WithByteLength(0,32))                                                                                                           
+                            && exists x:uint256 :: Equal<uint256>(s.n.0, x as uint256)
+                            && s.n.1 == 32
+                            witness Uint((0,32))                                                                                                           
 
     // Strangely, if the prefix "make" is dropped by the following functions,
     // then inside this module Dafny is still able to correctly associate when,
     // for example, Uint8 is used as a type or as function, however outside this
     // module Dafny appears to consider Uint8 only a type and not a function.
     function method makeUint8(a:uint8): Uint8
-    ensures makeUint8(a).n.n == a as uint256;
+    ensures makeUint8(a).n.0 == a as uint256;
     {
         assert Equal<uint256>(a as uint256, a as uint256);
-        Uint(Uint256WithByteLength(a as uint256,1))
+        Uint((a as uint256,1))
     }
 
     function method makeUint16(a:uint16): Uint16
-    ensures makeUint16(a).n.n == a as uint256;
+    ensures makeUint16(a).n.0 == a as uint256;
     {
         assert Equal<uint256>(a as uint256, a as uint256);
         assert a as nat < power2(16);
-        Uint(Uint256WithByteLength(a as uint256,2))
+        Uint((a as uint256,2))
     }    
 
     function method makeUint32(a:uint32): Uint32
-    ensures makeUint32(a).n.n == a as uint256;
+    ensures makeUint32(a).n.0 == a as uint256;
     {
         assert Equal<uint256>(a as uint256, a as uint256);
         assert a as nat < power2(32);
-        Uint(Uint256WithByteLength(a as uint256,4))
+        Uint((a as uint256,4))
     }
 
     function method makeUint64(a:uint64): Uint64
-    ensures makeUint64(a).n.n == castUin64ToUint256(a);
+    ensures makeUint64(a).n.0 == castUin64ToUint256(a);
     {
         assert Equal<uint256>(castUin64ToUint256(a),castUin64ToUint256(a));
         UpperBoundForUint64(a);
-        Uint(Uint256WithByteLength(a as uint256,8))
+        Uint((a as uint256,8))
     }  
 
     function method makeUint128(a:uint128): Uint128
-    ensures makeUint128(a).n.n == castUin128ToUint256(a);
+    ensures makeUint128(a).n.0 == castUin128ToUint256(a);
     {
         assert Equal<uint256>(castUin128ToUint256(a),castUin128ToUint256(a));
         UpperBoundForUint128(a);
-        Uint(Uint256WithByteLength(a as uint256,16))
+        Uint((a as uint256,16))
     } 
 
     function method makeUint256(a:uint256): Uint256
-    ensures makeUint256(a).n.n == a;
+    ensures makeUint256(a).n.0 == a;
     {
         assert Equal<uint256>(a as uint256, a as uint256);
-        Uint(Uint256WithByteLength(a,32))
+        Uint((a,32))
     }  
 
     /** The type `Bytes32` corresponding to a Serialisable built using the
@@ -193,7 +191,7 @@ module Eth2Types {
             match s 
                 case Bool(_) => Bool_
         
-                case Uint(n) => Uint_(n.byteLength)
+                case Uint(n) => Uint_(n.1)
 
                 case Bitlist(_) => Bitlist_
 
